Isabelle/Shelley/Finite_Map_Extras.thy
@@ -1,10 +1,10 @@
-section \<open> Extra features for \<open>fmap\<close>'s \<close>
+section \<open> Extra Features for Finite Maps \<close>
 
 theory Finite_Map_Extras
   imports "HOL-Library.Finite_Map"
 begin
 
-text \<open> Some extra lemmas and syntactic sugar for \<open>fmap\<close> \<close>
+text \<open> Extra lemmas and syntactic sugar for \<open>fmap\<close> \<close>
 
 abbreviation fmap_update (\<open>_'(_ $$:= _')\<close> [1000,0,0] 1000) where
   "fmap_update m k v \<equiv> fmupd k v m"
@@ -27,6 +27,81 @@ proof -
     by (simp add: Ball_def_raw domIff fmsubset.rep_eq map_le_def)
 qed
 
+lemma fmadd_singletons_comm:
+  assumes "k\<^sub>1 \<noteq> k\<^sub>2"
+  shows "{k\<^sub>1 $$:= v\<^sub>1} ++\<^sub>f {k\<^sub>2 $$:= v\<^sub>2} = {k\<^sub>2 $$:= v\<^sub>2} ++\<^sub>f {k\<^sub>1 $$:= v\<^sub>1}"
+proof (intro fmap_ext)
+  fix k
+  consider
+    (a) "k = k\<^sub>1" |
+    (b) "k = k\<^sub>2" |
+    (c) "k \<noteq> k\<^sub>1 \<and> k \<noteq> k\<^sub>2"
+    by auto
+  with assms show "({k\<^sub>1 $$:= v\<^sub>1} ++\<^sub>f {k\<^sub>2 $$:= v\<^sub>2}) $$ k = ({k\<^sub>2 $$:= v\<^sub>2} ++\<^sub>f {k\<^sub>1 $$:= v\<^sub>1}) $$ k"
+    by auto
+qed
+
+lemma fmap_singleton_comm:
+  assumes "m $$ k = None"
+  shows "m ++\<^sub>f {k $$:= v} = {k $$:= v} ++\<^sub>f m"
+  using assms
+proof (induction m arbitrary: k v rule: fmap_induct)
+  case fmempty
+  then show ?case
+    by simp
+next
+  case (fmupd x y m)
+  have "m(x $$:= y) ++\<^sub>f {k $$:= v} = m ++\<^sub>f {x $$:= y} ++\<^sub>f {k $$:= v}"
+    by simp
+  also from fmupd.hyps and fmupd.IH have "\<dots> = {x $$:= y} ++\<^sub>f m ++\<^sub>f {k $$:= v}"
+    by simp
+  also from fmupd.prems and fmupd.hyps and fmupd.IH have "\<dots> = {x $$:= y} ++\<^sub>f {k $$:= v} ++\<^sub>f m"
+    by (metis fmadd_assoc fmupd_lookup)
+  also have "\<dots> = {k $$:= v} ++\<^sub>f m(x $$:= y)"
+  proof (cases "x \<noteq> k")
+    case True
+    then have "{x $$:= y} ++\<^sub>f {k $$:= v} ++\<^sub>f m = {k $$:= v} ++\<^sub>f {x $$:= y} ++\<^sub>f m"
+      using fmadd_singletons_comm by metis
+    also from fmupd.prems and fmupd.hyps and fmupd.IH have "\<dots> = {k $$:= v} ++\<^sub>f m ++\<^sub>f {x $$:= y}"
+      by (metis fmadd_assoc)
+    finally show ?thesis
+      by simp
+  next
+    case False
+    with fmupd.prems show ?thesis
+      by auto
+  qed
+  finally show ?case .
+qed
+
+lemma fmap_disj_comm:
+  assumes "fmdom' m\<^sub>1 \<inter> fmdom' m\<^sub>2 = {}"
+  shows "m\<^sub>1 ++\<^sub>f m\<^sub>2 = m\<^sub>2 ++\<^sub>f m\<^sub>1"
+  using assms
+proof (induction m\<^sub>2 arbitrary: m\<^sub>1 rule: fmap_induct)
+  case fmempty
+  then show ?case
+    by simp
+next
+  case (fmupd k v m\<^sub>2)
+  then show ?case
+  proof (cases "m\<^sub>1 $$ k = None")
+    case True
+    from fmupd.hyps have "m\<^sub>1 ++\<^sub>f m\<^sub>2(k $$:= v) = m\<^sub>1 ++\<^sub>f m\<^sub>2 ++\<^sub>f {k $$:= v}"
+      by simp
+    also from fmupd.prems and fmupd.hyps and fmupd.IH have "\<dots> = m\<^sub>2 ++\<^sub>f m\<^sub>1 ++\<^sub>f {k $$:= v}"
+      by simp
+    also from True have "\<dots> = m\<^sub>2 ++\<^sub>f {k $$:= v} ++\<^sub>f m\<^sub>1"
+      using fmap_singleton_comm by (metis fmadd_assoc)
+    finally show ?thesis
+      by simp
+  next
+    case False
+    then show ?thesis
+      using fmupd.prems by auto
+  qed
+qed
+
 text \<open> Domain restriction \<close>
 
 abbreviation dom_res :: "'a set \<Rightarrow> ('a, 'b) fmap \<Rightarrow> ('a, 'b) fmap" (infixl \<open>\<lhd>\<close> 150) where
@@ -36,5 +111,52 @@ text \<open> Domain exclusion \<close>
 
 abbreviation dom_exc :: "'a set \<Rightarrow> ('a, 'b) fmap \<Rightarrow> ('a, 'b) fmap" (infixl \<open>\<lhd>'/\<close> 150) where
   "s \<lhd>/ m \<equiv> fmfilter (\<lambda>x. x \<notin> s) m"
+
+text \<open> Extra lemmas for \<open>\<lhd>\<close> and \<open>\<lhd>/\<close> \<close>
+
+lemma dom_exc_add_distr:
+  shows "s \<lhd>/ (m\<^sub>1 ++\<^sub>f m\<^sub>2) = (s \<lhd>/ m\<^sub>1) ++\<^sub>f (s \<lhd>/ m\<^sub>2)"
+  by (blast intro: fmfilter_add_distrib)
+
+lemma fmap_partition:
+  shows "m = s \<lhd>/ m ++\<^sub>f s \<lhd> m"
+proof (induction m rule: fmap_induct)
+  case fmempty
+  then show ?case
+    by simp
+next
+  case (fmupd k v m)
+  from fmupd.hyps have "s \<lhd>/ m(k $$:= v) ++\<^sub>f s \<lhd> m(k $$:= v) =
+    s \<lhd>/ (m ++\<^sub>f {k $$:= v}) ++\<^sub>f s \<lhd> (m ++\<^sub>f {k $$:= v})"
+    by simp
+  also have "\<dots> = s \<lhd>/ m ++\<^sub>f s \<lhd>/ {k $$:= v} ++\<^sub>f s \<lhd> m ++\<^sub>f s \<lhd> {k $$:= v}"
+    using dom_exc_add_distr by simp
+  finally show ?case
+  proof (cases "k \<in> s")
+    case True
+    then have "s \<lhd>/ m ++\<^sub>f s \<lhd>/ {k $$:= v} ++\<^sub>f s \<lhd> m ++\<^sub>f s \<lhd> {k $$:= v} =
+      s \<lhd>/ m ++\<^sub>f {$$} ++\<^sub>f s \<lhd> m ++\<^sub>f {k $$:= v}"
+      by simp
+    also have "\<dots> = s \<lhd>/ m ++\<^sub>f s \<lhd> m ++\<^sub>f {k $$:= v}"
+      by simp
+    also from fmupd.IH have "\<dots> = m ++\<^sub>f {k $$:= v}"
+      by simp
+    finally show ?thesis using fmupd.hyps
+      by auto
+  next
+    case False
+    then have "s \<lhd>/ m ++\<^sub>f s \<lhd>/ {k $$:= v} ++\<^sub>f s \<lhd> m ++\<^sub>f s \<lhd> {k $$:= v} =
+      s \<lhd>/ m ++\<^sub>f {k $$:= v} ++\<^sub>f s \<lhd> m ++\<^sub>f {$$}"
+      by simp
+    also have "\<dots> = s \<lhd>/ m ++\<^sub>f {k $$:= v} ++\<^sub>f s \<lhd> m"
+      by simp
+    also from fmupd.hyps have "\<dots> = s \<lhd>/ m ++\<^sub>f s \<lhd> m ++\<^sub>f {k $$:= v}"
+      using fmap_singleton_comm by (metis (full_types) fmadd_assoc fmlookup_filter)
+    also from fmupd.IH have "\<dots> = m ++\<^sub>f {k $$:= v}"
+      by simp
+    finally show ?thesis
+      by auto
+  qed
+qed
 
 end
