Isabelle/Shelley/Properties.thy
@@ -1,0 +1,194 @@
+section \<open> Properties \<close>
+
+theory Properties
+  imports UTxO
+begin
+
+subsection \<open> Preservation of Value \<close>
+
+text \<open> Lovelace Value \<close>
+
+fun val_coin :: "coin \<Rightarrow> coin" where
+  "val_coin c = c"
+
+abbreviation val_map :: "('a, coin) fmap \<Rightarrow> coin" where
+  "val_map m \<equiv> (\<Sum>k \<in> fmdom' m. m $$! k)"
+
+abbreviation val_utxo :: "utxo \<Rightarrow> coin" where
+  "val_utxo utxo \<equiv> ubalance utxo"
+
+fun val_utxo_state :: "utxo_state \<Rightarrow> coin" where
+  "val_utxo_state (utxo, deps, fees, _) = val_utxo utxo + deps + fees"
+
+lemma val_map_add:
+  assumes "k \<notin> fmdom' m"
+  shows "val_map m(k $$:= c) = val_map m + c"
+proof -
+  let ?m' = "m(k $$:= c)"
+  have "val_map ?m' = (\<Sum>k\<^sub>i \<in> fmdom' m \<union> {k}. ?m' $$! k\<^sub>i)"
+    by simp
+  also from assms have "\<dots> = (\<Sum>k\<^sub>i \<in> fmdom' m. ?m' $$! k\<^sub>i) + (?m' $$! k)"
+    by simp
+  also have "\<dots> = (\<Sum>k\<^sub>i \<in> fmdom' m. ?m' $$! k\<^sub>i) + c"
+    by simp
+  also from assms have "\<dots> = (\<Sum>k\<^sub>i \<in> fmdom' m. m $$! k\<^sub>i) + c"
+    by (metis (no_types, lifting) fmupd_lookup sum.cong)
+  finally show ?thesis
+    by simp
+qed
+
+lemma val_map_union:
+  assumes "fmdom' m\<^sub>1 \<inter> fmdom' m\<^sub>2 = {}"
+  shows "val_map (m\<^sub>1 ++\<^sub>f m\<^sub>2) = val_map m\<^sub>1 + val_map m\<^sub>2"
+  using assms
+proof (induction m\<^sub>2 arbitrary: m\<^sub>1 rule: fmap_induct)
+  case fmempty
+  then show ?case
+    by simp
+next
+  case (fmupd k c m\<^sub>2)
+  have "val_map (m\<^sub>1 ++\<^sub>f m\<^sub>2(k $$:= c)) = val_map ((m\<^sub>1 ++\<^sub>f m\<^sub>2)(k $$:= c))"
+    by simp
+  also have "\<dots> = val_map (m\<^sub>1 ++\<^sub>f m\<^sub>2) + c"
+  proof -
+    have "fmdom' (m\<^sub>1 ++\<^sub>f m\<^sub>2) = fmdom' m\<^sub>1 \<union> fmdom' m\<^sub>2"
+      by simp
+    moreover from fmupd.prems have "k \<notin> fmdom' m\<^sub>1"
+      by auto
+    moreover from fmupd.hyps have "k \<notin> fmdom' m\<^sub>2"
+      by (simp add: fmdom'_notI)
+    ultimately have "k \<notin> fmdom' (m\<^sub>1 ++\<^sub>f m\<^sub>2)"
+      by simp
+    then show ?thesis
+      using val_map_add by (metis sum.cong)
+  qed
+  also from fmupd.prems and fmupd.IH have "\<dots> = val_map m\<^sub>1 + val_map m\<^sub>2 + c"
+    by simp
+  also have "\<dots> = val_map m\<^sub>1 + val_map (m\<^sub>2(k $$:= c))"
+  proof -
+    from fmupd.hyps have "k \<notin> fmdom' m\<^sub>2"
+      by (simp add: fmdom'_notI)
+    then show ?thesis
+      using val_map_add by (metis (full_types) add.assoc)
+  qed
+  finally show ?case .
+qed
+
+text \<open>
+  NOTE: The precondition \<open>s \<subseteq> fmdom' m\<close> stated in the document is not really needed.
+\<close>
+lemma val_map_split:
+  shows "val_map m = val_map (s \<lhd>/ m) + val_map (s \<lhd> m)"
+proof -
+  have *: "fmdom' (s \<lhd>/ m) \<inter> fmdom' (s \<lhd> m) = {}"
+    by auto
+  then have "m = s \<lhd>/ m ++\<^sub>f s \<lhd> m"
+    using fmap_partition by simp
+  with * show ?thesis
+    using val_map_union by metis
+qed
+
+lemma val_utxo_val_map:
+  shows "val_utxo utxo = val_map (fmmap snd utxo)"
+proof -
+  have "fmdom' (fmmap snd utxo) = fmdom' utxo"
+    by simp
+  moreover have "\<And>k. k \<in> fmdom' utxo \<Longrightarrow> (fmmap snd utxo) $$! k = snd (utxo $$! k)"
+    using fmlookup_dom'_iff by force
+  ultimately show ?thesis
+    by auto
+qed
+
+text \<open>
+  NOTE:
+  \<^item> The proof in the document applies lemmas 15.3 and 15.4 on \<open>utxo\<close>'s,
+    however this is incorrect since the range of \<open>utxo\<close> is not \<open>coin\<close> but
+    \<open>(addr, coin)\<close>.
+  \<^item> The proof in the document applies lemma 15.4 without proving its
+    precondition, which is not trivial to formalize.
+  \<^item> This formalization does not rely on Theorem 15.10 (the proof in the document does).
+\<close>
+lemma utxo_value_preservation:
+  assumes "\<Gamma> \<turnstile> s \<rightarrow>\<^bsub>UTXO\<^esub>{tx} s'"
+  shows "val_utxo_state s + wbalance (txwdrls tx) = val_utxo_state s'"
+proof -
+  from assms show ?thesis
+  proof cases
+    case (utxo_inductive utxo pp stk_creds stpools refunded decayed deposit_change ups' ups slot gen_delegs deps fees)
+    from utxo_inductive(3) have "val_utxo_state s' =
+      val_utxo_state (
+        (txins tx \<lhd>/ utxo) ++\<^sub>f outs tx,
+        deps + deposit_change,
+        fees + txfee tx + decayed,
+        ups')"
+      by blast
+    also have "\<dots> =
+      ubalance ((txins tx \<lhd>/ utxo) ++\<^sub>f outs tx)
+      + (deps + deposit_change)
+      + (fees + txfee tx + decayed)"
+      by simp
+    also have "\<dots> =
+      ubalance (txins tx \<lhd>/ utxo) + ubalance (outs tx)
+      + (deps + deposit_change)
+      + (fees + txfee tx + decayed)"
+    proof -
+      have "ubalance ((txins tx \<lhd>/ utxo) ++\<^sub>f outs tx) =
+        val_map (fmmap snd ((txins tx \<lhd>/ utxo) ++\<^sub>f outs tx))"
+        by (fact val_utxo_val_map)
+      also have "\<dots> = val_map (fmmap snd (txins tx \<lhd>/ utxo) ++\<^sub>f fmmap snd (outs tx))"
+        by simp
+      also have "\<dots> = val_map (fmmap snd (txins tx \<lhd>/ utxo)) + val_map (fmmap snd (outs tx))"
+      proof -
+        from utxo_inductive(4) have "fmdom'(txins tx \<lhd>/ utxo) \<inter> fmdom' (outs tx) = {}"
+          using txins_outs_exc by blast
+        then show ?thesis
+          using val_map_union by (smt fmdom'_map sum.cong)
+      qed
+      also have "\<dots> = ubalance (txins tx \<lhd>/ utxo) + ubalance (outs tx)"
+        using val_utxo_val_map by presburger
+      finally show ?thesis
+        by linarith
+    qed
+    also from utxo_inductive(11) have "\<dots> =
+      ubalance (txins tx \<lhd>/ utxo) + ubalance (outs tx)
+      + (deps + deposits pp stpools (txcerts tx) - (refunded + decayed))
+      + (fees + txfee tx + decayed)"
+      by simp
+    also have "\<dots> =
+      ubalance (txins tx \<lhd>/ utxo) + ubalance (outs tx)
+      + deps + deposits pp stpools (txcerts tx) - refunded
+      + fees + txfee tx"
+      by simp
+    also from utxo_inductive(9) have "\<dots> =
+      ubalance (txins tx \<lhd>/ utxo) + ubalance (outs tx)
+      + deps + deposits pp stpools (txcerts tx) - key_refunds pp stk_creds tx
+      + fees + txfee tx"
+      by simp
+    also from utxo_inductive(7) have "\<dots> =
+      ubalance (txins tx \<lhd>/ utxo) + ubalance (txins tx \<lhd> utxo)
+      + wbalance (txwdrls tx) + key_refunds pp stk_creds tx
+      + deps - key_refunds pp stk_creds tx + fees"
+      by simp
+    also have "\<dots> =
+      ubalance (txins tx \<lhd>/ utxo) + ubalance (txins tx \<lhd> utxo)
+      + wbalance (txwdrls tx) + deps + fees"
+      by simp
+    also have "\<dots> = ubalance utxo + wbalance (txwdrls tx) + deps + fees"
+    proof -
+      have "ubalance (txins tx \<lhd>/ utxo) + ubalance (txins tx \<lhd> utxo) =
+        val_map (fmmap snd (txins tx \<lhd>/ utxo)) + val_map (fmmap snd (txins tx \<lhd> utxo))"
+        using val_utxo_val_map by presburger
+      also have "\<dots> =
+        val_map (txins tx \<lhd>/ (fmmap snd utxo)) + val_map (txins tx \<lhd> (fmmap snd utxo))"
+        by simp
+      also from utxo_inductive(6) have "\<dots> = val_map (fmmap snd utxo)"
+        using val_map_split by (metis fmdom'_map)
+      finally show ?thesis
+        using val_utxo_val_map by simp
+    qed
+    finally show ?thesis
+      using utxo_inductive(2) by simp
+  qed
+qed
+
+end
